books/projects/rp-rewriter/proofs/extract-formula-lemmas.lisp
@@ -310,17 +310,18 @@
    (defthm-insert-iff-to-force
      (defthm rp-evl-of-insert-off-to-force-lemma
        (if iff-flg
-           (iff (rp-evl (insert-iff-to-force term iff-flg) a)
+           (iff (rp-evl (insert-iff-to-force term rule-name iff-flg) a)
                 (rp-evl term a))
-         (equal (rp-evl (insert-iff-to-force term iff-flg) a)
+         (equal (rp-evl (insert-iff-to-force term rule-name iff-flg) a)
                 (rp-evl term a)))
        :flag insert-iff-to-force)
      (defthm rp-evl-lst-of-insert-off-to-force-lst
-       (equal (rp-evl-lst (insert-iff-to-force-lst lst) a)
+       (equal (rp-evl-lst (insert-iff-to-force-lst lst rule-name) a)
               (rp-evl-lst lst a))
        :flag insert-iff-to-force-lst)
      :hints (("Goal"
-              :in-theory (e/d (RP-EVL-OF-FNCALL-ARGS)
+              :in-theory (e/d (RP-EVL-OF-FNCALL-ARGS
+                               force$)
                               ((:definition rp-termp)
                                (:definition falist-consistent)
                                (:rewrite rp-evl-of-rp-equal2)
@@ -329,9 +330,9 @@
                                (:type-prescription insert-iff-to-force))))))
 
    (defthm rp-evl-of-insert-off-to-force
-     (and (iff (rp-evl (insert-iff-to-force term t) a)
+     (and (iff (rp-evl (insert-iff-to-force term rule-name t) a)
                (rp-evl term a))
-          (equal (rp-evl (insert-iff-to-force term nil) a)
+          (equal (rp-evl (insert-iff-to-force term rule-name nil) a)
                  (rp-evl term a)))
      :hints (("Goal"
               :use ((:instance rp-evl-of-insert-off-to-force-lemma
